The multiparticle kets representing the position and the state of the system are
\begin{gather*}
    \ket{\ve R} \equiv \ket{\ve r_1} \otimes ... \otimes \ket{\ve r_N} \\
    \ket{\ve \phi_H} \equiv \ket{\phi_1} \otimes ... \otimes \ket{\phi_N}
\end{gather*}
where $\ket{\ve r_i}$ represents the position of the particle $i$ and $\ket{\ve \phi_i}$ is the i-th orbital ket. \\
The single particle position kets are orthonormal, hence
\begin{equation*}
    \bracket{\ve r_i}{\ve r_j} = \delta_{ij} 
    \bracket{R'}{R} = \prod_{i=1}^N \delta_{ii'}
\end{equation*}
and the same holds for the state kets
\begin{gather*}
    \bracket{\phi_i}{\phi_j} = \delta_{ij} \\
    \bracket{\Phi_H'}{\Phi_H} = \left(\bra{\phi_1'} \otimes ... \otimes \bra{\phi_N'}\right)\left(\ket{\phi_1} \otimes ... \otimes \ket{\phi_N}\right) = \prod_{i=1}^N \delta_{ii'}
\end{gather*}
The action of the permutation operator on the position ket $\ket{\ve R}$ reads
\begin{align*}
    P_{ij}\ket{\ve R} = P_{ij} \ &\ket{\ve r_1} \otimes ...  \otimes \ket{\ve r_i} \otimes ... \otimes \ket{\ve r_j} \otimes ... \otimes \ket{\ve r_N} = \\
    = &\ket{\ve r_1} \otimes ...  \otimes \ket{\ve r_j} \otimes ... \otimes \ket{\ve r_i} \otimes ... \otimes \ket{\ve r_N}
\end{align*}
and the action on the ket $\ket{\Phi_H}$ can be obtained by introducing a completeness relation $\int \ket{\ve R}\bra{\ve R}$ so that
\begin{gather*}
   \bra{\ve{R'}}P_{ij}\ket{\ve \Phi_H} = \int \bra{\ve R'}P_{ij}\ket{\ve R}\bra{\ve R}\ket{\ve \Phi_H} = \\
   = \int \delta_{11'}...\delta_{ij'}...\delta_{ji'}...\delta_{NN'} \ \phi_1(\ve r_1)...\phi_i(\ve r_i)...\phi_j(\ve r_j)...\phi_N(\ve r_N) = \\
   \int \phi_1(\ve r_1)...\phi_i(\ve r_j)...\phi_j(\ve r_i)...\phi_N(\ve r_N)
\end{gather*}
Hence
\begin{gather*}
    \bracketOP{\Phi_H}{\Phi_H}{h_k P_{ij}} = \int\int \bra{\Phi_H}\ket{\ve R}\bra{\ve R}h_kP_{ij}\ket{\ve R'}\bracket{\ve R'}{\Phi_H} = \\ 
    = \int \phi_i^*(\ve r_j) \phi_j(\ve r_i) \ \phi_k^*(\ve r_k)h_k\phi_k(\ve r_k) = \delta_{ij} \int \phi_k^*(\ve r_k)h_k\phi_k(\ve r_k)
\end{gather*}
proving that the identity is the only permutation that gives non-zero terms in Eq.\,\ref{eq:permutation_to_identity}.